src/tactics/FStar.Tactics.Basic.fsi
@@ -43,11 +43,11 @@ val tacprint  : string -> unit
 val tacprint1 : string -> string -> unit
 val tacprint2 : string -> string -> string -> unit
 val tacprint3 : string -> string -> string -> string -> unit
-val print           : string -> tac<unit>
-val debug           : string -> tac<unit>
+val print     : string -> tac<unit>
 val dump_proofstate : proofstate -> string -> unit
 val print_proof_state1 : string -> tac<unit>
 val print_proof_state  : string -> tac<unit>
+val debugging : unit -> tac<bool>
 
 val fail : string -> tac<'a>
 val trivial : unit -> tac<unit>
