ulib/FStar.Tactics.Builtins.fst
@@ -164,9 +164,9 @@ assume val apply_lemma : term -> Tac unit
 of printing [str] on the compiler's standard output. *)
 assume val print : string -> Tac unit
 
-(** [debug str] is similar to [print str], but will only print the message
-if the [--debug] option was given for the current module. *)
-assume val debug : string -> Tac unit
+(** [debugging ()] returns true if the current module has the debug flag
+on, i.e. when [--debug MyModule] was passed in. *)
+assume val debugging : unit -> Tac bool
 
 (** Similar to [print], but will dump a text representation of the proofstate
 along with the message. *)
